Add the logical relation

theories/logrel.v
@@ -1,4 +1,180 @@
 Require Import Autosubst2.core Autosubst2.fintype Autosubst2.syntax.
+Require Import fp_red.
+From Hammer Require Import Tactics.
+From Equations Require Import Equations.
+Require Import ssreflect.
+Require Import Logic.PropExtensionality (propositional_extensionality).
+From stdpp Require Import relations (rtc(..)).
 Definition ProdSpace {n} (PA : Tm n -> Prop)
   (PF : Tm n -> (Tm n -> Prop) -> Prop) : Tm n -> Prop :=
   fun b => forall a PB, PA a -> PF a PB -> PB (App b a).
+
+Reserved Notation "⟦ A ⟧ i ;; I ↘ S" (at level 70).
+Inductive InterpExt {n} i (I : forall n, nat -> Tm n -> Prop) : Tm n -> (Tm n -> Prop) -> Prop :=
+| InterpExt_Fun A B PA PF :
+  ⟦ A ⟧ i ;; I ↘ PA ->
+  (forall a, PA a -> exists PB, PF a PB) ->
+  (forall a PB, PF a PB -> ⟦ subst_Tm (scons a VarTm) B ⟧ i ;; I ↘ PB) ->
+  ⟦ Pi A B ⟧ i ;; I ↘ (ProdSpace PA PF)
+
+| InterpExt_Univ j :
+  j < i ->
+  ⟦ Univ j ⟧ i ;; I ↘ (I n j)
+
+| InterpExt_Step A A0 PA :
+  RPar.R A A0 ->
+  ⟦ A0 ⟧ i ;; I ↘ PA ->
+  ⟦ A ⟧ i ;; I ↘ PA
+where "⟦ A ⟧ i ;; I ↘ S" := (InterpExt i I A S).
+
+Lemma InterpExt_Univ' {n} i  I j (PF : Tm n -> Prop) :
+  PF = I n j ->
+  j < i ->
+  ⟦ Univ j ⟧ i ;; I ↘ PF.
+Proof. hauto lq:on ctrs:InterpExt. Qed.
+
+Infix "<?" := Compare_dec.lt_dec (at level 60).
+
+Equations InterpUnivN n (i : nat) : Tm n -> (Tm n -> Prop) -> Prop by wf i lt :=
+  InterpUnivN n i := @InterpExt n i
+                     (fun n j A =>
+                        match j <? i  with
+                        | left _ => exists PA, InterpUnivN n j A PA
+                        | right _ => False
+                        end).
+Arguments InterpUnivN {n}.
+
+Lemma InterpExt_lt_impl {n : nat} i I I' A (PA : Tm n -> Prop) :
+  (forall j, j < i -> I n j = I' n j) ->
+  ⟦ A ⟧ i ;; I ↘ PA ->
+  ⟦ A ⟧ i ;; I' ↘ PA.
+Proof.
+  move => hI h.
+  elim : A PA /h.
+  - hauto lq:on rew:off ctrs:InterpExt.
+  - hauto q:on ctrs:InterpExt.
+  - hauto lq:on ctrs:InterpExt.
+Qed.
+
+Lemma InterpExt_lt_eq {n : nat} i I I' A (PA : Tm n -> Prop) :
+  (forall j, j < i -> I n j = I' n j) ->
+  ⟦ A ⟧ i ;; I ↘ PA =
+  ⟦ A ⟧ i ;; I' ↘ PA.
+Proof.
+  move => hI. apply propositional_extensionality.
+  have : forall j, j < i -> I' n j = I n j by sfirstorder.
+  firstorder using InterpExt_lt_impl.
+Qed.
+
+Notation "⟦ A ⟧ i ↘ S" := (InterpUnivN i A S) (at level 70).
+
+Lemma InterpUnivN_nolt n i :
+  @InterpUnivN n i = @InterpExt n i (fun n j (A : Tm n) => exists PA, ⟦ A ⟧ j ↘ PA).
+Proof.
+  simp InterpUnivN.
+  extensionality A. extensionality PA.
+  set I0 := (fun _ => _).
+  set I1 := (fun _ => _).
+  apply InterpExt_lt_eq.
+  hauto q:on.
+Qed.
+
+#[export]Hint Rewrite @InterpUnivN_nolt : InterpUniv.
+
+Lemma RPar_substone n (a b : Tm (S n)) (c : Tm n):
+    RPar.R a b -> RPar.R (subst_Tm (scons c VarTm) a) (subst_Tm (scons c VarTm) b).
+  Proof. hauto l:on inv:option use:RPar.substing, RPar.refl. Qed.
+
+Lemma InterpExt_Fun_inv n i I (A : Tm n) B P
+  (h :  ⟦ Pi A B ⟧ i ;; I ↘ P) :
+  exists (PA : Tm n -> Prop) (PF : Tm n -> (Tm n -> Prop) -> Prop),
+     ⟦ A ⟧ i ;; I ↘ PA /\
+    (forall a, PA a -> exists PB, PF a PB) /\
+    (forall a PB, PF a PB -> ⟦ subst_Tm (scons a VarTm) B ⟧ i ;; I ↘ PB) /\
+    P = ProdSpace PA PF.
+Proof.
+  move E : (Pi A B) h => T h.
+  move : A B E.
+  elim : T P / h => //.
+  - hauto l:on.
+  - move => A A0 PA hA hA0 hPi A1 B ?. subst.
+    elim /RPar.inv : hA => //= _ A2 A3 B0 B1 hA1 hB0 [*]. subst.
+    hauto lq:on ctrs:InterpExt use:RPar_substone.
+Qed.
+
+Lemma InterpExt_Fun_nopf n i I (A : Tm n) B PA  :
+  ⟦ A ⟧ i ;; I ↘ PA ->
+  (forall a, PA a -> exists PB, ⟦ subst_Tm (scons a VarTm) B ⟧ i ;; I ↘  PB) ->
+  ⟦ Pi A B ⟧ i ;; I ↘ (ProdSpace PA (fun a PB => ⟦ subst_Tm (scons a VarTm) B ⟧ i ;; I ↘ PB)).
+Proof.
+  move => h0 h1. apply InterpExt_Fun =>//.
+Qed.
+
+Lemma InterpUnivN_Fun_nopf n i (A : Tm n) B PA :
+  ⟦ A ⟧ i ↘ PA ->
+  (forall a, PA a -> exists PB, ⟦ subst_Tm (scons a VarTm) B ⟧ i ↘ PB) ->
+  ⟦ Pi A B ⟧ i ↘ (ProdSpace PA (fun a PB => ⟦ subst_Tm (scons a VarTm) B ⟧ i ↘ PB)).
+Proof.
+  hauto l:on use:InterpExt_Fun_nopf rew:db:InterpUniv.
+Qed.
+
+Lemma InterpExt_cumulative n i j I (A : Tm n) PA :
+  i < j ->
+   ⟦ A ⟧ i ;; I ↘ PA ->
+   ⟦ A ⟧ j ;; I ↘ PA.
+Proof.
+  move => h h0.
+  elim : A PA /h0;
+    hauto l:on ctrs:InterpExt use:PeanoNat.Nat.lt_trans.
+Qed.
+
+Lemma InterpUnivN_cumulative n i (A : Tm n) PA :
+   ⟦ A ⟧ i ↘ PA -> forall j, i < j ->
+   ⟦ A ⟧ j ↘ PA.
+Proof.
+  hauto l:on rew:db:InterpUniv use:InterpExt_cumulative.
+Qed.
+
+Lemma InterpExt_preservation n i I (A : Tm n) B P (h : InterpExt i I A P) :
+  RPar.R A B ->
+  ⟦ B ⟧ i ;; I ↘ P.
+Proof.
+  move : B.
+  elim : A P / h; auto.
+  - move => A B PA PF hPA ihPA hPB hPB' ihPB T hT.
+    elim /RPar.inv :  hT => //.
+    move => hPar A0 A1 B0 B1 h0 h1 [? ?] ?; subst.
+    apply InterpExt_Fun; auto.
+    move => a PB hPB0.
+    apply : ihPB; eauto.
+    sfirstorder use:RPar.cong, RPar.refl.
+  - hauto lq:on inv:RPar.R ctrs:InterpExt.
+  - move => A B P h0 h1 ih1 C hC.
+    have [D [h2 h3]] := RPar_diamond  _ _ _ _ h0 hC.
+    hauto lq:on ctrs:InterpExt.
+Qed.
+
+Lemma InterpUnivN_preservation n i (A : Tm n) B P (h : ⟦ A ⟧ i ↘ P) :
+  RPar.R A B ->
+  ⟦ B ⟧ i ↘ P.
+Proof. hauto l:on rew:db:InterpUnivN use: InterpExt_preservation. Qed.
+
+Lemma InterpExt_back_preservation_star n i I (A : Tm n) B P (h : ⟦ B ⟧ i ;; I ↘ P) :
+  rtc RPar.R A B ->
+  ⟦ A ⟧ i ;; I ↘ P.
+Proof. induction 1; hauto l:on ctrs:InterpExt. Qed.
+
+Lemma InterpExt_preservation_star n i I (A : Tm n) B P (h : ⟦ A ⟧ i ;; I ↘ P) :
+  rtc RPar.R A B ->
+  ⟦ B ⟧ i ;; I ↘ P.
+Proof. induction 1; hauto l:on use:InterpExt_preservation. Qed.
+
+Lemma InterpUnivN_preservation_star n i (A : Tm n) B P (h : ⟦ A ⟧ i ↘ P) :
+  rtc RPar.R A B ->
+  ⟦ B ⟧ i ↘ P.
+Proof. hauto l:on rew:db:InterpUnivN use:InterpExt_preservation_star. Qed.
+
+Lemma InterpUnivN_back_preservation_star n i (A : Tm n) B P (h : ⟦ B ⟧ i ↘ P) :
+  rtc RPar.R A B ->
+  ⟦ A ⟧ i ↘ P.
+Proof. hauto l:on rew:db:InterpUnivN use:InterpExt_back_preservation_star. Qed.
